new top-level similarity relation ~ with main lemma but -->* and k[(\e)0] axiom

LambdaLetToDollar.v
@@ -14,6 +14,7 @@ Reserved Notation "j' ~ⱼ j" (at level 40).
 Reserved Notation "k' ~ₖ k" (at level 40).
 Reserved Notation "t' ~ₜ t" (at level 40).
 Notation "↑ e" := (↑ e) (in custom λ_dollar_scope at level 0).
+Notation "↑ e" := (↑ e) (in custom λ_let_dollar_scope at level 0).
 
 Inductive sim_tm {A} : tm' A → tm A → Prop :=
 | sim_var  : ∀ a,
@@ -32,7 +33,7 @@ Inductive sim_tm {A} : tm' A → tm A → Prop :=
 | sim_eta  : ∀ (v' : val' A) (v : val A), v' ~ₑ v →
     v' ~ₑ <{ λ {liftV v} $ 0 }>
 | sim_beta : ∀ (v' : val' A) (v : val A) e' e, v' ~ₑ v → e' ~ₑ e →
-    <| λ {liftV' v'} $ e' |> ~ₑ <{ λ {liftV v} $ ↑(λ e) 0 }>
+    <| λ {liftV' v'} $ e' |> ~ₑ <{ λ {liftV v} $ ↑(λ e) 0 }> (* todo: k [↑(λ e) 0] *)
 (* | sim_eta_dol : ∀ (v1 v2 : val A) (v1' v2' : val' A),
     v1 ~ₑ v1' → v2 ~ₑ v2' → <{ v1 $ v2 }> ~ₑ <| v1' v2' |> *)
 | sim_let_fun : ∀ e1' e2' e1 e2, e1' ~ₑ e1 → e2' ~ₑ e2 →
@@ -82,6 +83,52 @@ Global Hint Constructors sim_T : core.
 Global Hint Constructors sim_val : core.
 Global Hint Constructors sim_non : core.
 Global Hint Constructors sim_tm : core.
+
+Axiom sim_beta_k : ∀ {A} (v' : val' A) (v : val A) k' k e' e,
+  v' ~ₑ v →
+  k' ~ₖ k →
+  e' ~ₑ e →
+  <| λ {liftV' v'} $ k'[e'] |> ~ₑ <{ λ {liftV v} $ k [↑(λ e) 0] }>.
+
+Reserved Notation "e' ~' e" (at level 40).
+Inductive sim' : tm' ␀ → tm ␀ → Prop :=
+| sim_assoc'  : ∀ k0' k0 t0' t0 v' v k' k j' j,
+    k0' ~ₖ k0 →
+    t0' ~ₜ t0 →
+    v' ~ᵥ v →
+    k' ~ₖ k →
+    j' ~ⱼ j →
+    <| k0'[t0'[let S₀ v' in ↑k'[↑j'[0]]]] |> ~' <{ k0[t0[k[j[S₀ {liftV v} 0]]]] }>
+| sim_assoc_let'  : ∀ k0' k0 t0' t0 v' v k' k e' e,
+    k0' ~ₖ k0 →
+    t0' ~ₜ t0 →
+    v' ~ᵥ v →
+    k' ~ₖ k →
+    e' ~ₑ e →
+    <| k0'[t0'[let S₀ v' in ↑k'[e']]] |> ~' <{ k0[t0[k[(λ e) (S₀ {liftV v} 0)]]] }>
+where "e' ~' e" := (sim' e' e).
+Global Hint Constructors sim' : core.
+
+Reserved Notation "e' ~ e" (at level 40).
+Inductive sim : tm' ␀ → tm ␀ → Prop :=
+| sim_sim_tm : ∀ e' e, e' ~ₑ e → e' ~ e
+| sim_assoc  : ∀ e' e, e' ~' e → e' ~ e
+(* | sim_assoc  : ∀ k0' k0 t0' t0 v' v k' k j' j,
+    k0' ~ₖ k0 →
+    t0' ~ₜ t0 →
+    v' ~ᵥ v →
+    k' ~ₖ k →
+    j' ~ⱼ j →
+    <| k0'[t0'[let S₀ v' in ↑k'[↑j'[0]]]] |> ~ <{ k0[t0[k[j[S₀ {liftV v} 0]]]] }>
+| sim_assoc_let  : ∀ k0' k0 t0' t0 v' v k' k e' e,
+    k0' ~ₖ k0 →
+    t0' ~ₜ t0 →
+    v' ~ᵥ v →
+    k' ~ₖ k →
+    e' ~ₑ e →
+    <| k0'[t0'[let S₀ v' in ↑k'[e']]] |> ~ <{ k0[t0[k[(λ e) (S₀ {liftV v} 0)]]] }> *)
+where "e' ~ e" := (sim e' e).
+Global Hint Constructors sim : core.
 
 Fixpoint let_to_dollar {A} (e : tm' A) : tm A :=
   match e with
@@ -213,6 +260,27 @@ Proof.
   induction t'; intros; inversion H; clear H; subst; cbn; auto.
   constructor; auto.
   apply sim_plug_k; auto.
+Qed.
+
+Lemma plug_k_compose : ∀ {A} {k1' : K' A} {k1 k2' k2},
+  k1' ~ₖ k1 →
+  k2' ~ₖ k2 →
+  ∃ k' k,
+    k' ~ₖ k /\
+    (∀ e', <| k1' [k2' [e']] |> = <| k' [e'] |>) /\
+    (∀ e , <{ k1  [k2  [e ]] }> = <{ k  [e ] }>).
+Proof with auto.
+  induction k1'; intros k1 k2' k2 Hk1 Hk2; inversion Hk1; clear Hk1; subst; cbn.
+  - repeat eexists...
+  - destruct (IHk1' _ _ _ H3 Hk2) as [k0' [k0 [Hk0 [Hsub1 Hsub2]]]].
+    exists (K_let' k0' <| ↑j'[0] |>), (K_cons j k0); repeat split; auto; intros;
+    try rewrite Hsub1;
+    try rewrite Hsub2...
+  - destruct (IHk1' _ _ _ H3 Hk2) as [k0' [k0 [Hk0 [Hsub1 Hsub2]]]].
+    exists (K_let' k0' t), (K_arg <{ λv e }> k0); repeat split; auto; intros;
+    try rewrite Hsub1;
+    try rewrite Hsub2...
+    constructor...
 Qed.
 
 Lemma sim_plug_k_inv : ∀ {A} (k' : K' A) e' term,
@@ -348,10 +416,113 @@ Lemma sim_lift_val : ∀ {A} {v' : val' A} {v},
 Admitted.
 Global Hint Resolve sim_lift_val : core.
 
-Theorem let_step_to_dollar_multi : ∀ e1' e2' e1,
+Lemma sim_lift_j : ∀ {A} {j' : J' A} {j},
+   j' ~ⱼ  j →
+  ↑j' ~ⱼ ↑j.
+Proof.
+  intros. inversion H; clear H; subst; cbn; auto.
+Qed.
+Global Hint Resolve sim_lift_j : core.
+
+Lemma sim_lift_k : ∀ {A} {k' : K' A} {k},
+   k' ~ₖ  k →
+  ↑k' ~ₖ ↑k.
+Admitted.
+Global Hint Resolve sim_lift_k : core.
+
+Lemma t_inv_inner : ∀ (t' : T' ␀) (t : T ␀),
+  t' ~ₜ t →
+  (t' = T_nil' /\ t = T_nil) \/
+  (∃ (t2' : T' ␀) (t2 : T ␀) (v' : val' ␀) (v : val ␀) (k' : K' ␀) (k : K ␀),
+    t2' ~ₜ t2 /\
+    v' ~ᵥ v /\
+    k' ~ₖ k /\
+    (∀ (e' : tm' ␀), <| t'[e'] |> = <| t2'[v' $ k'[e']] |>) /\
+    (∀ (e  : tm  ␀), <{ t [e ] }> = <{ t2 [v  $ k [e ]] }>)).
+Proof.
+  induction t'; intros. inversion H; clear H; subst; auto.
+  right.
+  inversion H; clear H; subst.
+  destruct (IHt' t0 H6) as [[Ht' Ht] | [t2' [t2 [v' [v_ [k' [k_ [Ht [Hv [Hk [Hplug' Hplug]]]]]]]]]]];
+  try solve [subst; repeat eexists; eauto].
+  inversion Hv; clear Hv; subst. rename H into Hv.
+  cbn.
+  exists (T_cons' v k t2'), (T_cons v0 k0 t2).
+  repeat eexists. auto. apply Hv. apply Hk.
+  intros. cbn. rewrite Hplug'; auto.
+  intros. cbn. rewrite Hplug; auto.
+Qed.
+
+Lemma k_inv_inner : ∀ (k' : K' ␀) (k : K ␀),
+  k' ~ₖ k →
+  (k' = K_nil' /\ k = K_nil) \/
+  (∃ (k2' : K' ␀) (k2 : K ␀) (j2' : J' ␀) (j2 : J ␀),
+    k2' ~ₖ k2 /\
+    j2' ~ⱼ j2 /\
+    (∀ (e' : tm' ␀), <| k'[e'] |> = <| k2'[let e' in ↑j2'[0]] |>) /\
+    (∀ (e  : tm  ␀), <{ k [e ] }> = <{ k2 [ j2[e]] }>)) \/
+  (∃ (k2' : K' ␀) (k2 : K ␀) (e2' : tm' ^␀) (e2 : tm ^␀),
+    k2' ~ₖ k2 /\
+    e2' ~ₑ e2 /\
+    (∀ (e' : tm' ␀), <| k'[e'] |> = <| k2'[let e' in e2'] |>) /\
+    (∀ (e  : tm  ␀), <{ k [e ] }> = <{ k2 [(λ e2) e] }>)).
+Proof with auto.
+  induction k'; intros; inversion H; clear H; subst; cbn; auto;
+  destruct (IHk' _ H4) as
+    [[Hk' Hk]
+    |[[k2' [k2 [j2' [j2 [Hk2 [Hj2 [Hke' Hke]]]]]]]
+     |[k2' [k2 [e2' [e2 [Hk2 [Hj2 [Hke' Hke]]]]]]]]]; subst; right.
+  - left. exists K_nil', K_nil. repeat eexists...
+  - left. exists (K_let' k2' <| ↑j'[0] |>), (K_cons j k2), j2', j2; repeat split; auto; intros.
+    + rewrite Hke' in *. reflexivity.
+    + rewrite Hke in *. reflexivity.
+  - right. exists (K_let' k2' <| ↑j'[0] |>), (K_cons j k2), e2', e2. repeat split; auto; intros; cbn.
+    + rewrite Hke' in *. reflexivity.
+    + rewrite Hke in *. reflexivity.
+  - right. exists K_nil', K_nil. repeat eexists...
+  - left. exists (K_let' k2' t), (K_arg <{ λv e }> k2), j2', j2. repeat split; auto; intros; cbn.
+    + constructor...
+    + rewrite Hke' in *. reflexivity.
+    + rewrite Hke in *. reflexivity.
+  - right. exists (K_let' k2' t), (K_arg <{ λv e }> k2), e2', e2. repeat split; auto; intros; cbn.
+    + constructor...
+    + rewrite Hke' in *. reflexivity.
+    + rewrite Hke in *. reflexivity.
+Qed.
+
+
+Lemma sim_plug_k' : ∀ k' k e' e,
+  k' ~ₖ k →
+  e' ~' e →
+  <| k'[e'] |> ~' <{ k[e] }>.
+Proof with auto.
+  intros. inversion H0; clear H0; subst.
+  - destruct (plug_k_compose H H1) as [k3' [k3 [Hk [Hsub1 Hsub2]]]]. rewrite Hsub1. rewrite Hsub2.
+    apply sim_assoc'...
+  - destruct (plug_k_compose H H1) as [k3' [k3 [Hk [Hsub1 Hsub2]]]]. rewrite Hsub1. rewrite Hsub2.
+    apply sim_assoc_let'...
+Qed.
+
+Lemma sim_plug_t' : ∀ t' t e' e,
+  t' ~ₜ t →
+  e' ~' e →
+  <| t'[e'] |> ~' <{ t[e] }>.
+Admitted.
+(* Proof with auto.
+  intros. inversion H0; clear H0; subst.
+  - destruct (t_inv_inner t' t H) as [[Hsub1 Hsub2]|[t2' [t2 [w' [w [k2' [k2 [Ht [Hw [Hk [Hsub1 Hsub2]]]]]]]]]]]; subst; cbn in *; auto.
+    rewrite Hsub1 in *.
+    rewrite Hsub2 in *.
+    clear Hsub1 Hsub2.
+    destruct (plug_k_compose Hk H1) as [k3' [k3 [Hk3 [Hsub1 Hsub2]]]]. rewrite Hsub1. rewrite Hsub2.
+    (* plug_k_compose *)
+Qed. *)
+
+
+Lemma let_step_to_dollar_multi_aux : ∀ e1' e2' e1,
   e1' -->' e2' →
   e1' ~ₑ e1 →
-  ∃  e3' e3, e2' -->'* e3' /\ e1 -->* e3 /\ e3' ~ₑ e3.
+  ∃  e3' e3, e2' -->'* e3' /\ e1 -->* e3 /\ e3' ~ e3.
 Proof with auto.
   intros term1' term2' term1 Hstep Hsim.
   inversion Hstep as [k' t' e1']; clear Hstep; subst. 
@@ -365,7 +536,7 @@ Proof with auto.
     repeat eexists.
     + auto.
     + eapply multi_k. eapply multi_t. apply Hmulti.
-    + apply sim_plug_k... apply sim_plug_t...
+    + apply sim_sim_tm. apply sim_plug_k... apply sim_plug_t...
   }
 
   (* redex_dollar' *)
@@ -373,7 +544,7 @@ Proof with auto.
     repeat eexists.
     + auto.
     + eapply multi_k. eapply multi_t. apply (multi_contr (contr_dollar _ _)).
-    + apply sim_plug_k... apply sim_plug_t...
+    + apply sim_sim_tm. apply sim_plug_k... apply sim_plug_t...
   }
 
   (* redex_shift' *)
@@ -389,39 +560,9 @@ Proof with auto.
       rewrite lambda_to_val.
       laws.
       apply multi_refl.
-    + apply sim_plug_k... apply sim_plug_t...
+    + apply sim_sim_tm. apply sim_plug_k... apply sim_plug_t...
       apply sim_app...
       constructor...
-    
-    (* inversion He; clear He; reason; subst. 
-    - apply sim_app_inv in H3 as [e1_3 [e1_4 [Hes [He2 Hsub]]]]; reason; subst.
-      eapply (sim_s_0_app _ v2) in Hes.
-      repeat eexists.
-      + eapply multi_k. eapply multi_t.
-        eapply multi_trans.
-        eapply multi_delim. apply Hes.
-        apply (multi_contr_multi (contr_shift v1 K_nil _)). cbn.
-        rewrite lambda_to_val.
-        laws.
-        apply multi_refl.
-      + apply sim_plug_k... apply sim_plug_t...
-        apply sim_app...
-        constructor...
-    - destruct v'; inversion H.
-    - clear v H.
-      rename v3 into v, v0 into w', v2 into w.
-    (* apply sim_dol_inv in He as [e1_1 [e1_2 [He1 [Hs Hsub]]]]; reason; subst. *)
-    (* apply sim_app_inv in Hs as [e1_3 [e1_4 [Hes [He2 Hsub]]]]; reason; subst. *)
-    (* eapply (sim_s_0_app _ v2) in Hes. *)
-    repeat eexists.
-    + eapply multi_k. eapply multi_t.
-      (* eapply multi_trans. *)
-      (* change <{ (λ e) (S₀ {liftV w} 0) }> with <{ {K_arg <{ λv e }> K_nil}[(S₀ {liftV w} 0)] }>. *)
-      (* apply contr_shift. *)
-      apply (multi_contr_multi (contr_shift _ (K_arg <{ λv e }> K_nil) <{ {liftV w} 0 }>)). cbn. laws.
-      apply multi_refl.
-    + apply sim_plug_k... apply sim_plug_t...
-      constructor... constructor... constructor... *)
   }
 
   (* redex_dol_let' *)
@@ -441,7 +582,7 @@ Proof with auto.
         cbn. laws.
         subst.
         auto.
-      + apply sim_plug_k... apply sim_plug_t... constructor...
+      + apply sim_sim_tm. apply sim_plug_k... apply sim_plug_t... constructor...
         change (val_to_tm (liftV <{ λv e2 }>)) with <{ ↑(λ e2) }>.
         apply sim_beta...
     * apply sim_app_inv in H1 as [es [e1_4 [Hes [He2 Hsub]]]]; reason; subst.
@@ -455,7 +596,7 @@ Proof with auto.
         eapply multi_contr_multi. apply (contr_shift _ (K_cons (J_fun _) K_nil)).
         cbn. laws.
         auto.
-      + apply sim_plug_k... apply sim_plug_t... repeat constructor...
+      + apply sim_sim_tm. apply sim_plug_k... apply sim_plug_t... repeat constructor...
     * apply sim_app_inv in H3 as [es [e1_4 [Hes [He2 Hsub]]]]; reason; subst.
       eapply sim_s_0_app in Hes.
       repeat eexists.
@@ -467,7 +608,7 @@ Proof with auto.
         eapply multi_contr_multi. apply (contr_shift _ (K_cons (J_arg _) K_nil)).
         cbn. laws.
         auto.
-      + apply sim_plug_k... apply sim_plug_t... repeat constructor...
+      + apply sim_sim_tm. apply sim_plug_k... apply sim_plug_t... repeat constructor...
     * apply sim_app_inv in H1 as [es [e1_4 [Hes [He2 Hsub]]]]; reason; subst.
       eapply sim_s_0_app in Hes.
       repeat eexists.
@@ -479,12 +620,12 @@ Proof with auto.
         eapply multi_contr_multi. apply (contr_shift _ (K_cons (J_dol _) K_nil)).
         cbn. laws.
         auto.
-      + apply sim_plug_k... apply sim_plug_t... repeat constructor...
+      + apply sim_sim_tm. apply sim_plug_k... apply sim_plug_t... repeat constructor...
   }
 
   (* redex_let' *)
   { repeat eexists; auto.
-    apply sim_plug_k... apply sim_plug_t...
+    apply sim_sim_tm. apply sim_plug_k... apply sim_plug_t...
     destruct j; cbn in *.
     - apply sim_app_inv in He as [n_ [e2 [He1 [He2 Hsub]]]]; reason; subst.
       apply sim_let_fun...
@@ -495,22 +636,172 @@ Proof with auto.
   }
 
   (* redex_let_beta' *)
-  { admit.
-    (* repeat eexists.
-    + auto.
-    + eapply multi_k. eapply multi_t. apply Hmulti.
-    + apply sim_plug_k... apply sim_plug_t... *)
+  { apply sim_let_inv in He as [[v_ [t0_ [H1 [H2 Hsub]]]]|[j' [j [v_ [Hv [Hj [Hsub1 Hsub2]]]]]]]; reason; subst.
+    - repeat eexists.
+      + auto.
+      + eapply multi_k. eapply multi_t. apply multi_contr. apply contr_beta.
+      + apply sim_sim_tm. apply sim_plug_k... apply sim_plug_t... apply sim_subst_lemma...
+    - rewrite subst_plug_of_lift_j.
+      repeat eexists.
+      + auto.
+      + eapply multi_k. eapply multi_t. eapply multi_j...
+      + apply sim_sim_tm. apply sim_plug_k... apply sim_plug_t... apply sim_plug_j...
   }
 
   (* redex_let_assoc' *)
-  { admit.
-    (* repeat eexists; auto.
-    apply sim_plug_k... apply sim_plug_t...
-    destruct (sim_let_inv _ _ _ He ) as [[x1 [x2 [Hx1 [Hx2 Hsub]]]]|[j' [j [x1 [Hx1 [Hj [Hsub1 Hsub2]]]]]]]; subst.
-    admit.
-    apply sim_let_fun.
-    destruct (sim_let_inv _ _ _ Hx1) as [[y1 [y2 [Hy1 [Hy2 Hsub]]]]|[j' [j [y1 [Hy1 [Hj [Hsub1 Hsub2]]]]]]]; subst.
-    inversion He; clear He; reason; subst.  *)
+  { destruct (sim_let_inv _ _ _ He ) as [[x1 [x2 [Hx1 [Hx2 Hsub]]]]|[j' [j [x1 [Hx1 [Hj [Hsub1 Hsub2]]]]]]]; subst.
+    * destruct (sim_let_inv _ _ _ Hx1) as [[y1 [y2 [Hy1 [Hy2 Hsub]]]]|[j0' [j0 [y1 [Hy1 [Hj0 [Hsub1 Hsub2]]]]]]]; subst.
+      + apply sim_app_inv in Hy1 as [es [v_ [Hes [Hv_ Hsub]]]]; reason; subst.
+        eapply (sim_s_0_app _ v0) in Hes.
+        repeat eexists.
+        - auto.
+        - eapply multi_k. eapply multi_t.
+          eapply (multi_j (J_arg <{ λv _ }>)). eapply (multi_j (J_arg <{ λv _ }>)). apply Hes.
+        - cbn.
+          rewrite lift_val_to_tm.
+          apply sim_assoc.
+          apply (sim_assoc_let' _ _ _ _ _ _ (K_let' K_nil' t1) (K_cons (J_arg <{ λv x2 }>) K_nil) t0 y2); auto.
+      + apply sim_app_inv in Hy1 as [es [v_ [Hes [Hv_ Hsub]]]]; reason; subst.
+        eapply (sim_s_0_app _ v0) in Hes.
+        repeat eexists.
+        - auto.
+        - eapply multi_k. eapply multi_t.
+          eapply (multi_j (J_arg <{ λv _ }>)). eapply multi_j. apply Hes.
+        - cbn.
+          rewrite lift_val_to_tm.
+          apply sim_assoc.
+          apply (sim_assoc' _ _ _ _ _ _ (K_let' K_nil' t1) (K_cons (J_arg <{ λv x2 }>) K_nil) j0' j0); auto.
+    * destruct (sim_let_inv _ _ _ Hx1) as [[y1 [y2 [Hy1 [Hy2 Hsub]]]]|[j0' [j0 [y1 [Hy1 [Hj0 [Hsub1 Hsub2]]]]]]]; subst.
+      + apply sim_app_inv in Hy1 as [es [v_ [Hes [Hv_ Hsub]]]]; reason; subst.
+        eapply (sim_s_0_app _ v0) in Hes.
+        repeat eexists.
+        - auto.
+        - eapply multi_k. eapply multi_t.
+          eapply multi_j. eapply (multi_j (J_arg <{ λv y2 }>)). apply Hes.
+        - cbn.
+          rewrite lift_val_to_tm.
+          apply sim_assoc.
+          apply (sim_assoc_let' _ _ _ _ _ _ (K_let' K_nil' <| ↑j'[0] |>) (K_cons j K_nil) t0 y2); auto.
+      + apply sim_app_inv in Hy1 as [es [v_ [Hes [Hv_ Hsub]]]]; reason; subst.
+        eapply (sim_s_0_app _ v0) in Hes.
+        repeat eexists.
+        - auto.
+        - eapply multi_k. eapply multi_t.
+          eapply multi_j. eapply multi_j. apply Hes.
+        - cbn.
+          rewrite lift_val_to_tm.
+          apply sim_assoc.
+          apply (sim_assoc' _ _ _ _ _ _ (K_let' K_nil' <| ↑j'[0] |>) (K_cons j K_nil) j0' j0); auto.
   }
-Admitted.
-(* Qed. *)
+(* Admitted. *)
+Qed.
+
+Lemma aux_K1 : ∀ k0' k0 v' v k' k j' j term',
+  k0' ~ₖ k0 →
+  v' ~ᵥ v →
+  k' ~ₖ k →
+  j' ~ⱼ j →
+  <| k0' [let S₀ v' in ↑k'[↑j'[0]]] |> -->' term' → ∃ term,
+  <{ k0  [k [j [S₀ {liftV v}   0]]] }> -->* term /\ term' ~' term.
+Proof with auto.
+  intros k0' k0 v' v k' k j' j term' Hk0 Hv Hk Hj Hstep.
+  destruct (k_inv_inner _ _ Hk0) as
+    [[Hke' Hke]
+    |[[k2' [k2 [j2' [j2 [Hk2 [Hj2 [Hke' Hke]]]]]]]
+      |[k2' [k2 [e2' [e2 [Hk2 [Hj2 [Hke' Hke]]]]]]]]].
+  * subst. cbn in *. apply let_S0_does_not_step in Hstep. destruct Hstep.
+  * repeat eexists; auto.
+    rewrite Hke' in *.
+    rewrite Hke in *.
+    apply plug_k_let_let_S0_step_inv in Hstep. subst.
+    apply (sim_assoc' k2' k2 T_nil' T_nil v' v (K_let' k' <| ↑j2'[0] |>) (K_cons j2 k))...
+  * repeat eexists; auto.
+    rewrite Hke' in *.
+    rewrite Hke in *.
+    apply plug_k_let_let_S0_step_inv in Hstep. subst.
+    apply (sim_assoc' k2' k2 T_nil' T_nil v' v (K_let' k' e2') (K_arg <{ λv e2 }> k))... constructor...
+Qed.
+
+Lemma aux_K2 : ∀ k0' k0 v' v k' k e' e term',
+  k0' ~ₖ k0 →
+  v' ~ᵥ v →
+  k' ~ₖ k →
+  e' ~ₑ e →
+  <| k0' [let S₀ v' in ↑k'[e']] |> -->' term' → ∃ term,
+  <{ k0  [k [(λ e) (S₀ {liftV v} 0)]] }> -->* term /\ term' ~' term.
+Proof with auto.
+  intros k0' k0 v' v k' k j' j term' Hk0 Hv Hk Hj Hstep.
+  destruct (k_inv_inner _ _ Hk0) as
+    [[Hke' Hke]
+    |[[k2' [k2 [j2' [j2 [Hk2 [Hj2 [Hke' Hke]]]]]]]
+      |[k2' [k2 [e2' [e2 [Hk2 [Hj2 [Hke' Hke]]]]]]]]].
+  * subst. cbn in *. apply let_S0_does_not_step in Hstep. destruct Hstep.
+  * repeat eexists; auto.
+    rewrite Hke' in *.
+    rewrite Hke in *.
+    apply plug_k_let_let_S0_step_inv in Hstep. subst.
+    apply (sim_assoc_let' k2' k2 T_nil' T_nil v' v (K_let' k' <| ↑j2'[0] |>) (K_cons j2 k))...
+  * repeat eexists; auto.
+    rewrite Hke' in *.
+    rewrite Hke in *.
+    apply plug_k_let_let_S0_step_inv in Hstep. subst.
+    apply (sim_assoc_let' k2' k2 T_nil' T_nil v' v (K_let' k' e2') (K_arg <{ λv e2 }> k))... constructor...
+Qed.
+
+Theorem let_step_to_dollar_multi : ∀ e1' e2' e1,
+  e1' -->' e2' →
+  e1' ~ e1 →
+  ∃  e3' e3, e2' -->'* e3' /\ e1 -->* e3 /\ e3' ~ e3.
+Proof with auto.
+  intros term1' term2' term1 Hstep Hsim.
+  inversion Hsim; clear Hsim; subst.
+  - apply (let_step_to_dollar_multi_aux _ _ _ Hstep H).
+  - inversion H; clear H; subst. 
+    { destruct (t_inv_inner _ _ H1) as [[Ht' Ht]|[t' [t [w' [w [kt' [kt [Ht [Hv [Hk [Hsub1 Hsub2]]]]]]]]]]]; subst; cbn in *.
+      + eapply aux_K1 in Hstep as [term [Hmulti Hsim]]; eauto.
+        repeat eexists. auto. apply Hmulti. apply (sim_assoc _ _ Hsim).
+      + rewrite Hsub1 in *.
+        rewrite Hsub2 in *.
+        apply plug_shift_step_inv' in Hstep as [inner [Hsub Hstep]]; subst.
+        apply shift_step_inv' in Hstep as [[Hkt Hsub]|[inner2 [Hstep Hsub]]]; subst; cbn in *.
+        * inversion Hk; clear Hk; subst; cbn in *.
+          clear Hsub1 Hsub2.
+          destruct (plug_k_compose H3 (sim_K_cons _ _ _ _ H4 sim_K_nil)) as [kj' [kj [Hkj [Hsub1 Hsub2]]]].
+          cbn in *.
+          rewrite Hsub2 in *.
+          repeat eexists.
+          - eapply multi_k'. eapply multi_t'. eapply multi_contr'. rewrite lambda_to_val'. apply contr_shift'.
+          - eapply multi_k. eapply multi_t. eapply multi_contr_multi. apply contr_shift.
+            cbn. laws. rewrite <- (lift_rewrite_plug_k_j _ _ _ Hsub2). auto.
+          - apply sim_sim_tm. apply sim_plug_k... apply sim_plug_t... repeat constructor... apply sim_plug_k... apply sim_plug_j...
+        * eapply aux_K1 in Hstep as [term [Hmulti Hsim]]; eauto.
+          repeat eexists.
+          - auto.
+          - eapply multi_k. eapply multi_t. eapply multi_delim. apply Hmulti.
+          - apply sim_assoc. eapply sim_plug_k'... eapply sim_plug_t'... eapply (sim_plug_t' (T_cons' w' K_nil' T_nil') (T_cons w K_nil T_nil))...
+    }
+    { destruct (t_inv_inner _ _ H1) as [[Ht' Ht]|[t' [t [w' [w [kt' [kt [Ht [Hv [Hk [Hsub1 Hsub2]]]]]]]]]]]; subst; cbn in *.
+      + eapply aux_K2 in Hstep as [term [Hmulti Hsim]]; eauto.
+        repeat eexists. auto. apply Hmulti. apply (sim_assoc _ _ Hsim).
+      + rewrite Hsub1 in *.
+        rewrite Hsub2 in *.
+        apply plug_shift_step_inv' in Hstep as [inner [Hsub Hstep]]; subst.
+        apply shift_step_inv' in Hstep as [[Hkt Hsub]|[inner2 [Hstep Hsub]]]; subst; cbn in *.
+        * inversion Hk; clear Hk; subst; cbn in *.
+          clear Hsub1 Hsub2.
+          destruct (plug_k_compose H3 (sim_K_let _ _ _ _ H4 sim_K_nil)) as [kj' [kj [Hkj [Hsub1 Hsub2]]]].
+          cbn in *.
+          rewrite Hsub2 in *.
+          repeat eexists.
+          - eapply multi_k'. eapply multi_t'. eapply multi_contr'. rewrite lambda_to_val'. apply contr_shift'.
+          - eapply multi_k. eapply multi_t. eapply multi_contr_multi. apply contr_shift.
+            cbn. laws. rewrite <- (lift_rewrite_plug_k_j _ (J_arg <{ λv e }>) _ Hsub2). cbn. auto.
+          - apply sim_sim_tm. apply sim_plug_k... apply sim_plug_t... constructor...
+            apply sim_beta_k...
+        * eapply aux_K2 in Hstep as [term [Hmulti Hsim]]; eauto.
+          repeat eexists.
+          - auto.
+          - eapply multi_k. eapply multi_t. eapply multi_delim. apply Hmulti.
+          - apply sim_assoc. eapply sim_plug_k'... eapply sim_plug_t'... eapply (sim_plug_t' (T_cons' w' K_nil' T_nil') (T_cons w K_nil T_nil))...
+    }
+Qed.
